o more fixing, working on rules for pi type.

per/per_props_admiss.v
@@ -34,31 +34,119 @@ Require Export nuprl_props.
 Require Export choice.
 Require Export cvterm.
 
+Hint Resolve iscvalue_mkc_admiss : slow.
+
+Lemma type_mkc_admiss {o} :
+  forall lib (A : @CTerm o), type lib (mkc_admiss A) <=> type lib A.
+Proof.
+  introv; split; intro h.
+
+  - unfold type in h; exrepnd.
+    inversion h0; subst; try not_univ.
+    allunfold_per; computes_to_value_isvalue; eauto 3 with slow.
+
+  - unfold type in h; exrepnd.
+    exists (per_admiss_eq eq).
+    apply CL_admiss.
+    exists A eq; dands; spcast; eauto 3 with slow.
+Qed.
+
+Definition cofinite_subst_fapprox {o}
+           lib
+           (T : @CTerm o)
+           {v : NVar}
+           (e e' : CVTerm [v])
+           (f : @CTerm o) :=
+    {j : nat
+     , forall (k :nat),
+         k>j -> equality lib (subst_fapproxc e f k) (subst_fapproxc e' f k) T}.
+
+Definition subst_fix {o}
+           lib
+           (T : @CTerm o)
+           {v : NVar}
+           (e e' : CVTerm [v])
+           (f : @CTerm o) :=
+  equality lib (subst_fixc e f) (subst_fixc e' f) T.
+
+Definition has_admissible_equality {o} lib (T : @CTerm o) :=
+  forall v (e e' : CVTerm [v]) (f : @CTerm o),
+    cofinite_subst_fapprox lib T e e' f
+    -> subst_fix lib T e e' f.
+
+Lemma admissible_equality_iff_has_admissible_equality {o} :
+  forall lib (A : @CTerm o) eq,
+    nuprl lib A eq
+    -> (admissible_equality eq <=> has_admissible_equality lib A).
+Proof.
+  introv n; split; introv h w.
+
+  - unfold subst_fix.
+    unfold cofinite_subst_fapprox in w; exrepnd.
+    eapply eq_equality0;[|eauto].
+    apply h.
+    unfold cofinite_subst_fapprox_eqc.
+    exists j.
+    introv gtk.
+    apply w0 in gtk.
+    eapply equality_implies_eq; eauto.
+
+  - unfold subst_fix_eqc.
+    unfold cofinite_subst_fapprox_eqc in w; exrepnd.
+    eapply equality_implies_eq;[eauto|].
+    apply h.
+    unfold cofinite_subst_fapprox.
+    exists j.
+    introv gtk.
+    apply w0 in gtk.
+    eapply eq_equality0;eauto.
+Qed.
+
+Lemma equality_in_mkc_admiss_iff_has_admissible_equality {o} :
+  forall lib (t u A : @CTerm o),
+    equality lib t u (mkc_admiss A) <=> (has_admissible_equality lib A # type lib A).
+Proof.
+  introv; split; intro h.
+
+  - unfold equality in h; exrepnd.
+    inversion h1; subst; try not_univ.
+    match goal with
+    | [ H : per_admiss _ _ _ _ |- _ ] => rename H into q
+    end.
+    allunfold @per_admiss; exrepnd.
+    computes_to_value_isvalue.
+    fold (nuprl lib) in *.
+    apply q1 in h0; unfold per_admiss_eq in h0.
+    dands; eauto 3 with slow.
+    eapply admissible_equality_iff_has_admissible_equality; eauto.
+
+  - repnd.
+    unfold type in h; exrepnd.
+    exists (per_admiss_eq eq); dands; auto.
+    { apply CL_admiss.
+      exists A eq; dands; spcast; eauto 3 with slow. }
+    unfold per_admiss_eq.
+    eapply admissible_equality_iff_has_admissible_equality; eauto.
+Qed.
 
 Lemma tequality_admiss {p} :
   forall lib (A1 A2 : @CTerm p),
     tequality lib (mkc_admiss A1) (mkc_admiss A2)
-    <=> tequality lib A1 A2.
+    <=> (type lib A1
+         # type lib A2
+         # (has_admissible_equality lib A1 <=> has_admissible_equality lib A2)).
 Proof.
-  intros.
-  sp_iff Case.
+  introv.
+  rw @tequality_iff_ext_eq.
+  allrw @type_mkc_admiss.
 
-  - Case "->".
-    introv teq.
-    unfold tequality, nuprl in teq; exrepnd.
-    inversion teq0; subst; try not_univ.
-    allunfold @per_admiss; exrepnd.
-    computes_to_value_isvalue.
-    allfold @nuprl.
-    dands.
-    exists eqa; auto.
+  split; intro h; repnd; dands; auto.
 
-  - Case "<-".
-    intro teq.
-    unfold tequality in teq; destruct teq as [eqa n].
-    exists (per_admiss_eq lib eqa).
-    apply CL_admiss.
-    unfold per_admiss.
-    exists A1 A2 eqa; dands; fold @nuprl; auto;
-    try (complete (spcast; apply computes_to_valc_refl; apply_iscvalue)).
+  - pose proof (h mkc_axiom mkc_axiom) as q; clear h.
+    repeat (rw @equality_in_mkc_admiss_iff_has_admissible_equality in q).
+    split; intro w; destruct q as [q1 q2];[autodimp q1 hyp|autodimp q2 hyp];tcsp.
+
+  - introv.
+    repeat (rw @equality_in_mkc_admiss_iff_has_admissible_equality).
+    split; intro w; repnd; destruct h as [q1 q2];[autodimp q1 hyp|autodimp q2 hyp];tcsp.
 Qed.
