rules/rules_function.v
@@ -35,10 +35,12 @@ Require Export sequents_tacs.
 Require Export sequents_tacs2.
 Require Export rules_useful.
 Require Export per_props_equality.
+Require Export per_props_function.
 Require Export sequents_equality.
 Require Export rules_tyfam.
 Require Export subst_tacs_aeq.
 Require Export cequiv_tacs.
+
 
 (** printing |- $\vdash$ *)
 (** printing ->  $\rightarrow$ *)
@@ -271,582 +273,36 @@ Proof.
   - apply isprog_vars_comm; simpl; auto.
 Qed.
 
+Hint Rewrite @vars_hyps_substitute_hyps : slow.
 
-(* end hide *)
-
-(**
-
-  The Nuprl manual%~\cite{Kreitz:02}% presents various useful rules to
-  reason about function types.  This section prove the truth of
-  several of these rules.
-
-*)
-
-(* [17] ============ FUNCTION ELIMINATION ============ *)
-
-(**
-
- The following rule is called the function elimination rules.  It says
- that if we can prove that [a] is in the domain [A] then we can assume
- that [f a] is in [B[x\a]].  As for the other rules, first we show an
- informal statement of this rule, then we show its formal statement (a
- [Definition]), and finally we show the statement that the rule is
- true (a [Lemma]).  In such informal statements, we write ``C ext e''
- to indicate that e is the extract of the sequent, i.e., the evidence
- that C is true.  We omit the ``ext e'' part when e is [mk_axiom].
-
-<<
-   H, f : x:A->B[x], J |- C ext e[z\axiom]
-
-     By perFunctionElimination s z
-
-     H, f : x:A->B[x], J |- a in A
-     H, f : x:A->B[x], J, z : (f a) in B[a] |- C ext e
->>
-
- *)
-
-Definition rule_function_elimination_concl {o}
-           (A : @NTerm o) B C e f x z H J :=
-  mk_baresequent
-    (snoc H (mk_hyp f (mk_function A x B)) ++ J)
-    (mk_concl C (subst e z mk_axiom)).
-
-Definition rule_function_elimination_hyp1 {o}
-           (A : @NTerm o) B a ea f x H J :=
-  mk_baresequent
-    (snoc H (mk_hyp f (mk_function A x B)) ++ J)
-    (mk_concl (mk_member a A) ea).
-
-Definition rule_function_elimination_hyp2 {o}
-           (A : @NTerm o) B C a e f x z H J :=
-  mk_baresequent
-    (snoc (snoc H (mk_hyp f (mk_function A x B)) ++ J)
-          (mk_hyp z (mk_member (mk_apply (mk_var f) a)
-                               (subst B x a))))
-    (mk_concl C e).
-
-Definition rule_function_elimination {p}
-           (A B C a e : NTerm) ea
-           (f x z : NVar)
-           (H J : @barehypotheses p) :=
-  mk_rule
-    (rule_function_elimination_concl A B C e f x z H J)
-    [
-      rule_function_elimination_hyp1 A B a ea f x H J,
-      rule_function_elimination_hyp2 A B C a e f x z H J
-    ]
-    [(*sarg_term a, sarg_var z*)].
-
-Lemma rule_function_elimination_true3 {p} :
-  forall lib (A B C a e : NTerm) ea,
-  forall f x z : NVar,
-  forall H J : @barehypotheses p,
-    rule_true3 lib (rule_function_elimination
-                 A B C a e
-                 ea
-                 f x z
-                 H J).
+(* !!MOVE to per_props_equality.v *)
+Lemma implies_tequality_mkc_member_if_member {o} :
+  forall lib (a b A B : @CTerm o),
+    tequality lib A B
+    -> (forall x, equality lib x a A <=> equality lib x b B)
+    -> tequality lib (mkc_member a A) (mkc_member b B).
 Proof.
-  unfold rule_function_elimination, rule_true3, wf_bseq, closed_type_baresequent, closed_extract_baresequent; simpl.
-  intros; repnd.
-  clear cargs.
-
-  (* We prove the well-formedness of things *)
-  destseq; allsimpl.
-  dLin_hyp; exrepnd.
-  rename Hyp into hyp1.
-  rename Hyp0 into hyp2.
-  destruct hyp1 as [ ws1 hyp1 ].
-  destruct hyp2 as [ ws2 hyp2 ].
-  destseq; allsimpl; proof_irr; GC.
-
-  assert (wf_csequent (snoc H (mk_hyp f (mk_function A x B)) ++ J)
-                      ||- (mk_concl C (subst e z mk_axiom))) as wfc.
-  {
-    clear hyp1 hyp2.
-    unfold wf_csequent, closed_type, closed_extract, wf_sequent, wf_concl; simpl.
-    prove_seq; eauto 3 with slow.
-    apply covered_subst; eauto 2 with slow.
-    eapply covered_subvars;[|eauto].
-    autorewrite with slow; simpl.
-    rw subvars_eq; introv i; simpl.
-    repeat (allrw @in_snoc; allrw @in_app_iff).
-    repndors; tcsp.
-  }
-  exists wfc.
-  unfold wf_csequent, wf_sequent, wf_concl in wfc; allsimpl; repnd; proof_irr; GC.
-
-  (* We prove some simple facts on our sequents *)
-  assert (disjoint (free_vars A) (vars_hyps J)
-          # disjoint (remove_nvars [x] (free_vars B)) (vars_hyps J)
-          # subvars (free_vars a) (snoc (vars_hyps H) f ++ vars_hyps J)
-          # wf_term a
-          # !LIn z (free_vars C)
-          # !LIn z (vars_hyps H)
-          # !LIn z (vars_hyps J)
-          # (z <> f)
-          # !LIn f (vars_hyps H)
-          # !LIn f (vars_hyps J)
-          # !LIn f (free_vars A)
-          # (x <> f -> !LIn f (free_vars B))) as vhyps.
-  {
-    clear hyp1 hyp2.
-    dwfseq.
-    sp;
-      try (complete (introv i; discover; allunfold @disjoint; discover; auto));
-      try (complete (assert (LIn f (remove_nvars [x] (free_vars B)))
-                      by (rw in_remove_nvars; rw in_single_iff; sp);
-                     discover; auto));
-      try (complete (apply wf_member_iff in wfct0; sp));
-      try (complete (generalize (wfh10 z); rw in_app_iff; rw in_snoc; sp));
-      try (complete (generalize (wfh10 f); rw in_remove_nvars; simpl; intro i;
-                     dest_imp i hyp));
-      try complete (pose proof (wfc1 z) as xx; autodimp xx hyp;
-                    rw in_app_iff in xx; rw in_snoc in xx; repndors; tcsp).
-  }
-
-  destruct vhyps as [ daj vhyps ].
-  destruct vhyps as [ dbj vhyps ].
-  destruct vhyps as [ sva vhyps ].
-  destruct vhyps as [ wa vhyps ].
-  destruct vhyps as [ nizc vhyps ].
-  destruct vhyps as [ nizh vhyps ].
-  destruct vhyps as [ nizj vhyps ].
-  destruct vhyps as [ nzf vhyps ].
-  destruct vhyps as [ nifh vhyps ].
-  destruct vhyps as [ nifj vhyps ].
-  destruct vhyps as [ nifa nifb ].
-  (* done with proving these simple facts *)
-
-  vr_seq_true.
-
-  duplicate sim as simapp.
-
-  rw @similarity_app in sim; simpl in sim; exrepnd; subst; cpx.
-  rw @similarity_snoc in sim5; simpl in sim5; exrepnd; subst; cpx.
-  lsubst_tac.
-  rw @equality_in_function in sim2; repnd.
-
-  vr_seq_true in hyp2.
-  generalize (hyp2 (snoc (snoc s1a0 (f, t1) ++ s1b) (z, mkc_axiom))
-                   (snoc (snoc s2a0 (f, t2) ++ s2b) (z, mkc_axiom)));
-    clear hyp2; intros hyp2.
-  repeat (autodimp hyp2 h); exrepnd.
-
-  {
-    (* hyps_functionality *)
-
-    pose proof (hyps_functionality_snoc
-                  lib
-                  (snoc H (mk_hyp f (mk_function A x B)) ++ J)
-                  (mk_hyp z (mk_member (mk_apply (mk_var f) a) (subst B x a)))
-                  (snoc s1a0 (f, t1) ++ s1b)
-                  mkc_axiom) as k; simpl in k.
-    apply k; try (complete auto); clear k.
-    introv eq sim; GC; lsubst_tac.
-    rw @tequality_mkc_member_sp.
-    apply equality_refl in eq.
-    rw <- @member_member_iff in eq.
-
-    vr_seq_true in hyp1.
-    generalize (hyp1 (snoc s1a0 (f, t1) ++ s1b) s'); clear hyp1; intros hyp1.
-    repeat (autodimp hyp1 h); exrepnd.
-    lsubst_tac.
-    allapply @member_if_inhabited.
-    rw @tequality_mkc_member_sp in hyp0; repnd.
-
-    assert (equality lib (lsubstc a wa (snoc s1a0 (f, t1) ++ s1b) c3)
-                     (lsubstc a wa s' c5)
-                     (lsubstc A w1 s1a0 c1)) as eqa.
-    {
-      sp.
-      unfold member in hyp1.
-      spcast; apply @equality_respects_cequivc_right with (t2 := lsubstc a wa (snoc s1a0 (f, t1) ++ s1b) c3); sp.
-    }
-
-    applydup sim5 in eqa.
-
-    duplicate sim as sim'.
-    apply eqh in sim'.
-
-    rw @eq_hyps_app in sim'; simpl in sim'; exrepnd; subst; cpx.
-    apply app_split in sim'0; repnd; allrw length_snoc;
-    try (complete (allrw; sp)); subst; cpx.
-
-    rw @eq_hyps_snoc in sim'5; simpl in sim'5; exrepnd; subst; cpx.
-    lsubst_tac.
-    rw @tequality_function in sim'0; repnd.
-
-    applydup sim'0 in eqa as teq.
-
-    assert (disjoint (remove_nvars [x] (free_vars B)) (dom_csub s1b0)) as disj1.
-    {
-      apply similarity_dom in sim1; repnd.
-      rw sim7.
-      rewrite vars_hyps_substitute_hyps; auto.
-    }
-
-    assert (disjoint (remove_nvars [x] (free_vars B)) (dom_csub s2b0)) as disj2.
-    {
-      apply sub_eq_hyps_dom in sim'1; repnd.
-      rw sim'1; auto.
-    }
-
-    repeat (substc_lsubstc_vars3;[]).
-
-    dands.
-
-    {
-      repeat (lsubstc_subst_aeq2;[]).
-      repeat (substc_lsubstc_vars3;[]).
-      repeat (lsubstc_weak;[]).
-      proof_irr.
-      auto.
-    }
-
-    rw @similarity_app in sim; simpl in sim; exrepnd; subst; cpx.
-    apply app_split in sim7; repnd; allrw length_snoc;
-    try (complete (allrw; sp)); subst; cpx.
-    apply app_split in sim9; repnd; allrw length_snoc;
-    try (complete (allrw; sp)); subst; cpx.
-    rw @similarity_snoc in sim12; simpl in sim12; exrepnd; subst; cpx.
-    lsubst_tac.
-    rw @equality_in_function in sim9; repnd.
-    applydup sim9 in eqa as eqf.
-
-    left.
-    repeat (lsubstc_subst_aeq2;[]).
-    repeat (substc_lsubstc_vars3;[]).
-    repeat (lsubstc_weak;[]).
-    proof_irr.
-    auto.
-  }
-
-
-  {
-    (* similarity *)
-
-    assert (wf_term (mk_member (mk_apply (mk_var f) a) (subst B x a))) as wm.
-    {
-      apply wf_member; sp; try (apply wf_apply; sp).
-      apply subst_preserves_wf_term; sp.
-    }
-
-    assert (cover_vars (mk_member (mk_apply (mk_var f) a) (subst B x a))
-                       (snoc s1a0 (f, t1) ++ s1b)) as cm.
-    {
-      apply cover_vars_member; sp.
-      apply cover_vars_apply; sp.
-      apply cover_vars_var.
-      rw @dom_csub_app; rw @dom_csub_snoc; rw in_app_iff; rw in_snoc; simpl; sp.
-      rw @cover_vars_eq; rw @dom_csub_app; rw @dom_csub_snoc; insub.
-      (* begin proof of last cover_vars *)
-      rw @cover_vars_eq; rw @cover_vars_covered; apply covered_subst; sp.
-      rw @dom_csub_app; rw @dom_csub_snoc; simpl.
-      rw cons_app; apply covered_app_weak_l.
-      clear sim2 sim5; unfold cover_vars_upto in c2; unfold covered.
-      prove_subvars c2; allsimpl; sp.
-      rw @dom_csub_csub_filter in l; rw in_remove_nvars in l; rw in_single_iff in l.
-      rw in_snoc; sp.
-      clear hyp1; rw @covered_equality in ct0; repnd.
-      unfold covered; unfold covered in ct1.
-      rw @vars_hyps_app in ct1; rw @vars_hyps_snoc in ct1; simpl in ct1.
-      rw @dom_csub_app; rw @dom_csub_snoc; simpl.
-      allapply @similarity_dom; repnd; allrw; rw @vars_hyps_substitute_hyps; sp.
-      (* end proof of last cover_vars *)
-    }
-
-    sim_snoc.
-    dands; auto.
-    lsubst_tac.
-    rw @member_eq.
-    rw <- @member_member_iff.
-
-    vr_seq_true in hyp1.
-    generalize (hyp1 (snoc s1a0 (f, t1) ++ s1b)
-                     (snoc s2a0 (f, t2) ++ s2b));
-      clear hyp1; intros hyp1.
-    repeat (autodimp hyp1 h); exrepnd.
-    lsubst_tac.
-    allapply @member_if_inhabited.
-    rw @tequality_mkc_member_sp in hyp0; repnd.
-    unfold member in hyp1.
-    apply sim2 in hyp1.
-
-    assert (disjoint (remove_nvars [x] (free_vars B)) (dom_csub s1b)) as disj1.
-    {
-      apply similarity_dom in sim1; repnd.
-      rw sim7.
-      rewrite vars_hyps_substitute_hyps; auto.
-    }
-
-    apply equality_refl in hyp1.
-    unfold member in *.
-    repeat (lsubstc_subst_aeq2;[]).
-    repeat (substc_lsubstc_vars3;[]).
-    repeat (lsubstc_weak;[]).
-    proof_irr.
-    auto.
-  }
-
-  (* conclusion *)
-
-  lsubst_tac; sp.
-
-  assert (wf_term (@mk_axiom p)) as wfax by eauto 2 with slow.
-
-  repeat (lsubstc_subst_aeq2;[]).
-  allrw @lsubstc_mk_axiom.
-  repeat (substc_lsubstc_vars3;[]).
-  proof_irr.
-
-  pose proof (lsubstc_snoc_move
-                e
-                (snoc s1a0 (f, t1) ++ s1b)
-                []
-                z
-                mkc_axiom
-                wfce) as xx1.
-  allrw app_nil_r.
-  allrw @dom_csub_app.
-  allrw @dom_csub_snoc.
-  allsimpl.
-  pose proof (xx1 pt0) as xx2; clear xx1.
-  autodimp xx2 hyp.
-  { apply similarity_dom in sim6; repnd.
-    rewrite sim7.
-    apply similarity_dom in sim1; repnd.
-    rewrite sim8.
-    rewrite vars_hyps_substitute_hyps; auto.
-    rw in_app_iff; rw in_snoc; intro i; repndors; tcsp.
-  }
-  exrepnd.
-  proof_irr.
-  rewrite <- xx0; clear xx0.
-
-  pose proof (lsubstc_snoc_move
-                e
-                (snoc s2a0 (f, t2) ++ s2b)
-                []
-                z
-                mkc_axiom
-                wfce) as xx1.
-  allrw app_nil_r.
-  allrw @dom_csub_app.
-  allrw @dom_csub_snoc.
-  allsimpl.
-  pose proof (xx1 pt3) as xx2; clear xx1.
-  autodimp xx2 hyp.
-  { apply similarity_dom in sim6; repnd.
-    rewrite sim6.
-    apply similarity_dom in sim1; repnd.
-    rewrite sim1.
-    rewrite vars_hyps_substitute_hyps; auto.
-    rw in_app_iff; rw in_snoc; intro i; repndors; tcsp.
-  }
-  exrepnd.
-  proof_irr.
-  rewrite <- xx0; clear xx0.
-
-  auto.
+  introv teq equ.
+  apply tequality_mkc_member; dands; eauto 3 with slow.
+  introv; split; intro h; repnd; dands; eauto 3 with nequality; apply equ; auto.
 Qed.
 
-(* begin hide *)
-
-Lemma rule_function_elimination_true {p} :
-  forall lib (A B C a e : NTerm) ea,
-  forall f x z : NVar,
-  forall H J : @barehypotheses p,
-    rule_true lib (rule_function_elimination
-                     A B C a e
-                     ea
-                     f x z
-                     H J).
+(* !!MOVE to per_props_equality.v *)
+Lemma tequality_mkc_member_implies_equality {o} :
+  forall lib (a1 a2 A1 A2 : @CTerm o),
+    tequality lib (mkc_member a1 A1) (mkc_member a2 A2)
+    -> member lib a1 A1
+    -> equality lib a1 a2 A1.
 Proof.
-  introv.
-  apply rule_true3_implies_rule_true.
-  apply rule_function_elimination_true3.
+  introv teq mem.
+  apply tequality_mkc_member in teq; repnd.
+
+  pose proof (teq a1 a1 a1) as q; destruct q as [q q']; clear q'.
+  autodimp q hyp; repnd; dands; eauto 3 with nequality.
+
+  pose proof (teq a2 a2 a2) as w; destruct w as [w' w]; clear w'.
+  autodimp w hyp; repnd; dands; eauto 3 with nequality.
 Qed.
-
-Lemma rule_function_elimination_true2 {o} :
-  forall lib A B C a e ea f x z H J,
-    @rule_true2 o lib (rule_function_elimination A B C a e ea f x z H J).
-Proof.
-  intros.
-  apply rule_true_iff_rule_true2.
-  apply rule_function_elimination_true.
-Qed.
-
-Lemma rule_function_elimination_true_ex {p} :
-  forall lib (A B C a e : NTerm) ea,
-  forall f x z : NVar,
-  forall H J : @barehypotheses p,
-    rule_true_if lib (rule_function_elimination
-                        A B C a e
-                        ea
-                        f x z
-                        H J).
-Proof.
-  intros.
-  generalize (rule_function_elimination_true lib A B C a e ea f x z H J); intro rt.
-  rw <- @rule_true_eq_ex in rt.
-  unfold rule_true_ex in rt; sp.
-Qed.
-
-Lemma rule_function_elimination_wf {o} :
-  forall (A B C a e : @NTerm o) ea f x z H J,
-    wf_term a
-    -> covered a (snoc (vars_hyps H) f ++ vars_hyps J)
-    -> !LIn z (vars_hyps H)
-    -> !LIn z (vars_hyps J)
-    -> z <> f
-    -> wf_term ea
-    -> wf_rule (rule_function_elimination A B C a e ea f x z H J).
-Proof.
-  introv wa cov nizH nizJ dzf wea.
-
-  introv pwf m; allsimpl; repdors; subst; sp;
-  allunfold @pwf_sequent; wfseq; sp.
-
-  {
-    allrw @vswf_hypotheses_nil_eq.
-    allrw @wf_hypotheses_app; repnd.
-    allrw @wf_hypotheses_snoc; repnd.
-    allsimpl.
-    allapply @isprog_vars_implies_wf.
-    allrw <- @wf_function_iff; tcsp.
-  }
-
-  {
-    allrw @vswf_hypotheses_nil_eq.
-    allrw @wf_hypotheses_app; repnd.
-    allrw @wf_hypotheses_snoc; repnd.
-    allsimpl.
-    allapply @isprog_vars_implies_covered.
-    allrw @covered_function; repnd.
-    apply covered_snoc_app_weak.
-    apply covered_app_weak_l; auto.
-  }
-
-  {
-    allrw @vswf_hypotheses_nil_eq.
-    rw @wf_hypotheses_snoc; simpl; dands; tcsp.
-    - apply isprog_vars_member; dands.
-      + apply isprog_vars_apply; dands.
-        * apply isprog_vars_var_iff.
-          rw @vars_hyps_app.
-          rw @vars_hyps_snoc; simpl.
-          rw in_app_iff.
-          rw in_snoc; tcsp.
-        * rw @isprog_vars_iff_covered; dands; auto.
-          rw @vars_hyps_app.
-          rw @vars_hyps_snoc; simpl; auto.
-      + apply isprog_vars_subst2; auto.
-        * allrw @wf_hypotheses_app; repnd.
-          allrw @wf_hypotheses_snoc; repnd.
-          allsimpl.
-          allapply @isprog_vars_implies_wf.
-          allrw <- @wf_function_iff; tcsp.
-        * rw @isprog_vars_iff_covered; dands; auto.
-          rw @vars_hyps_app.
-          rw @vars_hyps_snoc; simpl; auto.
-        * allrw @wf_hypotheses_app; repnd.
-          allrw @wf_hypotheses_snoc; repnd.
-          allsimpl.
-          allrw <- @isprog_vars_function_iff; repnd.
-          allrw @vars_hyps_app.
-          allrw @vars_hyps_snoc; simpl.
-          eapply isprog_vars_subvars;[|eauto].
-          rw subvars_eq; introv i; allsimpl.
-          allrw in_app_iff; allrw in_snoc; tcsp.
-    - intro i.
-      allrw @vars_hyps_app.
-      allrw @vars_hyps_snoc; allsimpl.
-      allrw in_app_iff; allrw in_snoc.
-      repndors; tcsp.
-  }
-
-  {
-    allrw @wf_term_eq.
-    allrw @nt_wf_lsubst_iff; tcsp.
-  }
-
-  {
-    apply covered_snoc_weak; auto.
-  }
-Qed.
-
-Lemma rule_function_elimination_wf2 {o} :
-  forall (A B C a e : @NTerm o) ea f x z H J,
-    wf_term a
-    -> covered a (snoc (vars_hyps H) f ++ vars_hyps J)
-    -> !LIn z (vars_hyps H)
-    -> !LIn z (vars_hyps J)
-    -> z <> f
-    -> wf_rule2 (rule_function_elimination A B C a e ea f x z H J).
-Proof.
-  introv wa cova nizH nizJ dzf wf j.
-  allsimpl; repndors; subst; tcsp;
-  allunfold @wf_bseq; repnd; allsimpl; wfseq.
-
-  - allrw @vswf_hypotheses_nil_eq.
-    allrw @wf_hypotheses_app; repnd.
-    allrw @wf_hypotheses_snoc; repnd.
-    allapply @isprog_vars_implies_wf.
-    allrw <- @wf_function_iff; tcsp.
-
-  - allrw @vswf_hypotheses_nil_eq.
-    allrw @wf_hypotheses_app; repnd.
-    allrw @wf_hypotheses_snoc; repnd.
-    allapply @isprog_vars_implies_covered.
-    allrw @covered_function; repnd.
-    apply covered_snoc_app_weak.
-    apply covered_app_weak_l; auto.
-
-  - allrw @vswf_hypotheses_nil_eq.
-    rw @wf_hypotheses_snoc; simpl; dands; tcsp.
-    { apply isprog_vars_member; dands.
-      + apply isprog_vars_apply; dands.
-        * apply isprog_vars_var_iff.
-          rw @vars_hyps_app.
-          rw @vars_hyps_snoc; simpl.
-          rw in_app_iff.
-          rw in_snoc; tcsp.
-        * rw @isprog_vars_iff_covered; dands; auto.
-          rw @vars_hyps_app.
-          rw @vars_hyps_snoc; simpl; auto.
-      + apply isprog_vars_subst2; auto.
-        * allrw @wf_hypotheses_app; repnd.
-          allrw @wf_hypotheses_snoc; repnd.
-          allsimpl.
-          allapply @isprog_vars_implies_wf.
-          allrw <- @wf_function_iff; tcsp.
-        * rw @isprog_vars_iff_covered; dands; auto.
-          rw @vars_hyps_app.
-          rw @vars_hyps_snoc; simpl; auto.
-        * allrw @wf_hypotheses_app; repnd.
-          allrw @wf_hypotheses_snoc; repnd.
-          allsimpl.
-          allrw <- @isprog_vars_function_iff; repnd.
-          allrw @vars_hyps_app.
-          allrw @vars_hyps_snoc; simpl.
-          eapply isprog_vars_subvars;[|eauto].
-          rw subvars_eq; introv i; allsimpl.
-          allrw in_app_iff; allrw in_snoc; tcsp.
-    }
-    { intro i.
-      allrw @vars_hyps_app.
-      allrw @vars_hyps_snoc; allsimpl.
-      allrw in_app_iff; allrw in_snoc.
-      repndors; tcsp.
-    }
-
-  - apply covered_snoc_weak; auto.
-Qed.
-
-
-(* end hide *)
 
 
 (* [23] ============ LAMBDA FORMATION ============ *)
@@ -870,24 +326,24 @@ Qed.
  *)
 
 Definition rule_lambda_formation {p}
-           (A B b : NTerm)
+           (A B b e : NTerm)
            (x z  : NVar)
            (i    : nat)
            (H    : @barehypotheses p) :=
   mk_rule
     (mk_baresequent H (mk_concl (mk_function A x B) (mk_lam z b)))
     [ mk_baresequent (snoc H (mk_hyp z A))
-                    (mk_concl (subst B x (mk_var z)) b),
-      mk_baresequent H (mk_conclax (mk_equality A A (mk_uni i))) ]
+                     (mk_concl (subst B x (mk_var z)) b),
+      mk_baresequent H (mk_concl_eq_ext A A (mk_uni i) e) ]
     [sarg_var z].
 
 Lemma rule_lambda_formation_true {p} :
-  forall lib (A B b : NTerm)
+  forall lib (A B b e : NTerm)
          (x z : NVar)
          (i   : nat)
          (H   : @barehypotheses p)
          (bc1 : !LIn z (bound_vars B)),
-    rule_true lib (rule_lambda_formation A B b x z i H).
+    rule_true lib (rule_lambda_formation A B b e x z i H).
 Proof.
   intros.
   unfold rule_lambda_formation, rule_true, closed_type_baresequent, closed_extract_baresequent; simpl.
@@ -895,14 +351,9 @@ Proof.
 
   (* We prove the well-formedness of things *)
   destseq; allsimpl.
-  generalize (hyps (mk_baresequent (snoc H (mk_hyp z A))
-                                  (mk_concl (subst B x (mk_var z)) b))
-                   (inl eq_refl))
-             (hyps (mk_baresequent H (mk_conclax (mk_equality A A (mk_uni i))))
-                   (inr (inl eq_refl)));
-    simpl; intros hyp1 hyp2.
-  destruct hyp1 as [ ws1 hyp1 ].
-  destruct hyp2 as [ ws2 hyp2 ].
+  dLin_hyp; exrepnd.
+  rename Hyp0 into hyp1.
+  rename Hyp1 into hyp2.
   destseq; allsimpl; proof_irr; GC.
 
   allunfold @closed_type; allunfold @closed_extract; allsimpl.
@@ -913,10 +364,10 @@ Proof.
   allrw @nh_vars_hyps_snoc; allsimpl.
 
   assert (covered (mk_lam z b) (nh_vars_hyps H)) as cv.
-  clear hyp1 hyp2.
-  allunfold @covered; allsimpl; allrw app_nil_r.
-  allrw subvars_remove_nvars.
-  allrw <- snoc_as_append; sp.
+  { clear hyp1 hyp2.
+    allunfold @covered; allsimpl; allrw app_nil_r.
+    allrw subvars_remove_nvars.
+    allrw <- snoc_as_append; sp. }
 
   exists cv; GC.
 
@@ -924,17 +375,18 @@ Proof.
   assert ((z <> x -> !LIn z (free_vars B))
           # !LIn z (free_vars A)
           # !LIn z (vars_hyps H)) as vhyps.
-
-  clear hyp1 hyp2.
-  dwfseq.
-  sp;
-  try (complete (generalize (cg z); sp;
-                 allrw in_remove_nvars; allsimpl;
-                 autodimp X0 h; sp));
-  try (complete (apply_in_hyp p;
-                 generalize (subvars_hs_vars_hyps H); intro sv;
-                 rw subvars_prop in sv;
-                 apply sv in p; sp)).
+  {
+    clear hyp1 hyp2.
+    dwfseq.
+    sp;
+      try (complete (generalize (cg z); sp;
+                     allrw in_remove_nvars; allsimpl;
+                     autodimp X0 h; sp));
+      try (complete (apply_in_hyp p;
+                     generalize (subvars_hs_vars_hyps H); intro sv;
+                     rw subvars_prop in sv;
+                     apply sv in p; sp)).
+  }
 
   destruct vhyps as [ nzB vhyps ].
   destruct vhyps as [ nzA nzH ].
@@ -946,268 +398,276 @@ Proof.
   (* We prove our first subgoal *)
   assert (forall s2 pC2,
             similarity lib s1 s2 H
-            -> tequality lib (lsubstc (mk_function A x B) wfi s1 pC1)
-                         (lsubstc (mk_function A x B) wfi s2 pC2)) as tfb.
-  clear s2 pC2 pt2 sim.
-  intros s2 pC2 sim.
-  lift_lsubst.
-  rw @tequality_function.
+            -> tequality
+                 lib
+                 (lsubstc (mk_function A x B) wfi s1 pC1)
+                 (lsubstc (mk_function A x B) wfi s2 pC2)) as tfb.
+  {
+    clear s2 pC2 pt2 sim.
+    intros s2 pC2 sim.
+    lift_lsubst.
+    apply implies_tequality_function.
 
-  (* we have to prove that A is a type and B is a type family *)
-  split.
+    - vr_seq_true in hyp2.
+      pose proof (hyp2 s1 s2) as hyp2.
+      repeat (autodimp hyp2 h); exrepnd.
+      lsubst_tac.
+      allrw @fold_mkc_member.
+      apply equality_in_member in hyp2; exrepnd; eauto 3 with slow.
+      apply tequality_mkc_member_implies_equality in hyp0; eauto 3 with slow.
 
-  (* we use our 2nd hypothesis to prove that A is a type *)
-  vr_seq_true in hyp2.
-  generalize (hyp2 s1 s2); clear hyp2; intro hyp2.
-  autodimp hyp2 h.
-  autodimp hyp2 h; exrepd.
-  lsubst_tac.
-  rw @tequality_mkc_equality_sp in t; repnd; GC.
-  allrewrite @member_eq.
-  rw <- @member_equality_iff in e.
-  allapply @equality_in_uni.
-  destruct t1 as [ s | s ].
-  apply @equality_in_uni in s; auto.
-  spcast; apply tequality_respects_cequivc_right with (T2 := lsubstc A wa s1 c1); auto.
+    - (* we use our 1st hypothesis to prove that B is a type family *)
+      introv equ.
+      vr_seq_true in hyp1.
+      generalize (hyp1 (snoc s1 (z, a)) (snoc s2 (z, a'))); clear hyp1; intro hyp1.
+      autodimp hyp1 h.
 
-  (* we use our 1st hypothesis to prove that B is a type family *)
-  intros.
-  vr_seq_true in hyp1.
-  generalize (hyp1 (snoc s1 (z, a)) (snoc s2 (z, a'))); clear hyp1; intro hyp1.
-  autodimp hyp1 h.
+      {
+        (* To use our 1st hyp, we first have to prove that the hypotheses are functional *)
+        intros s3 sim3.
+        inversion sim3; cpx; allsimpl; cpx; clear_irr.
+        assert (cover_vars A s4) as c4
+            by (apply similarity_cover_vars with (t := A) in sim0; auto).
+        (* we use our hyp (coming from proving that our sequent is true) that says that H is functional *)
+        rw @eq_hyps_snoc; simpl.
 
-  (* To use our 1st hyp, we first have to prove that the hypotheses are functional *)
-  intros s3 sim3.
-  inversion sim3; cpx; allsimpl; cpx; clear_irr.
-  assert (cover_vars A s4) as c4
-    by (apply similarity_cover_vars with (t := A) in sim0; auto).
-  (* we use our hyp (coming from proving that our sequent is true) that says that H is functional *)
-  rw @eq_hyps_snoc; simpl.
+        exists s1 s4 a t2 wa c1 c4; sp.
+        (* now to prove that functionality statement on A, we use our 2nd hyp *)
+        vr_seq_true in hyp2.
+        generalize (hyp2 s1 s4); clear hyp2; intro hyp2.
+        autodimp hyp2 hyp.
+        autodimp hyp2 hyp; exrepd.
+        lsubst_tac.
+        allrw @fold_mkc_member.
+        apply equality_in_member in e1; exrepnd; eauto 3 with slow.
+        eapply tequality_in_uni_implies_tequality in t; eauto 3 with slow.
+        apply equality_refl in e4.
+        apply t in e4; eauto 3 with slow.
+      }
+      (* and we're done proving that the hypotheses are functional *)
 
-  exists s1 s4 a t2 wa c1 c4; sp.
-  (* now to prove that functionality statement on A, we use our 2nd hyp *)
-  vr_seq_true in hyp2.
-  generalize (hyp2 s1 s4); clear hyp2; intro hyp2.
-  autodimp hyp2 hyp.
-  autodimp hyp2 hyp; exrepd.
-  lsubst_tac.
-  rw @tequality_mkc_equality_sp in t; repnd; GC.
-  allrewrite @member_eq.
-  allrw <- @member_equality_iff.
-  allapply @equality_in_uni.
-  destruct t1 as [ s | s ].
-  apply @equality_in_uni in s; auto.
-  spcast; apply tequality_respects_cequivc_right with (T2 := lsubstc A wa s1 c1); auto.
-  (* and we're done proving that the hypotheses are functional *)
+      (* now we can keep using our 1st hypothesis *)
+      autodimp hyp1 hyp.
 
-  (* now we can keep using our 1st hypothesis *)
-  autodimp hyp1 hyp.
+      {
+        (* For that we have to prove that the two terms we picked to be equal in A are actually equal in A *)
+        sim_snoc2; dands; auto; proof_irr; auto.
+      }
+      (* easy enough *)
 
-  (* For that we have to prove that the two terms we picked to be equal in A are actually equal in A *)
-  rw @similarity_snoc; simpl.
-  exists s1 s2 a a' wa c1; sp.
-  (* easy enough *)
+      (* and again, we keep on using our 1st hypothesis *)
+      exrepd. (* we prove that from t *)
 
-  (* and again, we keep on using our 1st hypothesis *)
-  exrepd. (* we prove that from t *)
+      assert (lsubstc (subst B x (mk_var z)) wfct1 (snoc s1 (z, a)) pC0
+              = substc a x (lsubstc_vars B wb (csub_filter s1 [x]) [x] c2)) as eq1
+          by (apply lsubstc_subst_snoc_eq; try (complete sp);
+              allapply @similarity_dom; exrepd; allrw; sp).
 
-  assert (lsubstc (subst B x (mk_var z)) wfct1 (snoc s1 (z, a)) pC0
-          = substc a x (lsubstc_vars B wb (csub_filter s1 [x]) [x] c2)) as eq1
-         by (apply lsubstc_subst_snoc_eq; try (complete sp);
-             allapply @similarity_dom; exrepd; allrw; sp).
+      rewrite eq1 in t.
 
-  rewrite eq1 in t.
+      assert (lsubstc (subst B x (mk_var z)) wfct1 (snoc s2 (z, a')) pC3
+              = substc a' x (lsubstc_vars B wb (csub_filter s2 [x]) [x] c3)) as eq2
+          by (apply lsubstc_subst_snoc_eq; try (complete sp);
+              allapply @similarity_dom; exrepd; allrw; sp).
 
-  assert (lsubstc (subst B x (mk_var z)) wfct1 (snoc s2 (z, a')) pC3
-          = substc a' x (lsubstc_vars B wb (csub_filter s2 [x]) [x] c3)) as eq2
-         by (apply lsubstc_subst_snoc_eq; try (complete sp);
-             allapply @similarity_dom; exrepd; allrw; sp).
-
-  rewrite eq2 in t.
-  auto.
-  (* and we're done proving our 1st subgoal (the tequality) *)
-
+      rewrite eq2 in t.
+      auto.
+      (* and we're done proving our 1st subgoal (the tequality) *)
+  }
 
   (* We now prove our second subgoal *)
-  sp; lift_lsubst.
+  dands; tcsp.
+  lift_lsubst.
   applydup @similarity_refl in sim.
   rw @equality_in_function.
 
-  sp.
+  dands.
   (* We have to prove 3 goals *)
 
-  (* 1) we have to prove that A is a type *)
-  generalize (tfb s1 pC1 sim0); sp.
-  lsubst_tac.
-  allrw @tequality_function; sp.
+  {
+    (* 1) we have to prove that A is a type *)
+    generalize (tfb s1 pC1 sim0); sp.
+    lsubst_tac.
+    allrw @tequality_function; sp.
+  }
 
-  (* 2) we have to prove that B is a type family *)
-  generalize (tfb s1 pC1 sim0); sp.
-  lsubst_tac.
-  allrw @tequality_function; sp.
+  {
+    (* 2) we have to prove that B is a type family *)
+    generalize (tfb s1 pC1 sim0); sp.
+    lsubst_tac.
+    allrw @tequality_function; sp.
+  }
 
-  (* 3) we have to prove that b is a member B *)
-  vr_seq_true in hyp1.
-  generalize (hyp1 (snoc s1 (z, a)) (snoc s2 (z, a'))); clear hyp1; intro hyp1.
-  autodimp hyp1 hyp.
+  {
+    (* 3) we have to prove that b is a member B *)
+    vr_seq_true in hyp1.
+    introv eqa.
+    generalize (hyp1 (snoc s1 (z, a)) (snoc s2 (z, a'))); clear hyp1; intro hyp1.
+    autodimp hyp1 hyp.
 
-  (* first we have to prove that the hypotheses are functional *)
-  intros s3 sim3.
-  inversion sim3; cpx; allsimpl; cpx; clear_irr.
-  assert (cover_vars A s4) as c4
-    by (apply similarity_cover_vars with (t := A) in sim1; auto).
-  (* we use our hyp (coming from proving that our sequent is true) that says that H is functional *)
-  allapplydup eqh.
-  rw @eq_hyps_snoc; simpl.
-  exists s1 s4 a t2 wa c1 c4; sp.
-  (* now to prove that functionality statement on A, we use our 2nd hyp (from tfb) *)
-  assert (cover_vars (mk_isect A x B) s4) as c5
-    by (apply cover_vars_isect; sp;
-        allapplydup @similarity_dom; sp;
-        apply @cover_vars_upto_eq_dom_csub with (s2 := s4) in c2; sp;
-        allrw; sp).
-  generalize (tfb s4 c5 sim1); sp.
-  lsubst_tac.
-  allrw @tequality_function; sp.
-  (* and we're done proving that the hypotheses are functional *)
+    {
+      (* first we have to prove that the hypotheses are functional *)
+      intros s3 sim3.
+      inversion sim3; cpx; allsimpl; cpx; clear_irr.
+      assert (cover_vars A s4) as c4
+          by (apply similarity_cover_vars with (t := A) in sim1; auto).
+      (* we use our hyp (coming from proving that our sequent is true) that says that H is functional *)
+      allapplydup eqh.
+      rw @eq_hyps_snoc; simpl.
+      exists s1 s4 a t2 wa c1 c4; sp.
+      (* now to prove that functionality statement on A, we use our 2nd hyp (from tfb) *)
 
-  (* now we can keep using our 1st hypothesis *)
-  autodimp hyp1 hyp.
+      vr_seq_true in hyp2.
+      pose proof (hyp2 s1 s4) as hyp2.
+      repeat (autodimp hyp2 hyp); exrepnd.
+      lsubst_tac.
+      allrw @fold_mkc_member.
+      apply equality_in_member in hyp1; exrepnd; eauto 3 with slow.
+      apply tequality_mkc_member_implies_equality in hyp0; eauto 3 with slow.
+      (* and we're done proving that the hypotheses are functional *)
+    }
 
-  (* For that we have to prove that the two terms we picked to be equal in A are actually equal in A *)
-  rw @similarity_snoc; simpl.
-  exists s1 s2 a a' wa c1; sp.
-  (* easy enough *)
+    (* now we can keep using our 1st hypothesis *)
+    autodimp hyp1 hyp.
 
-  (* and again, we keep on using our 1st hypothesis *)
-  exrepd. (* we prove that from e *)
-  clear t; clear_irr.
+    {
+      (* For that we have to prove that the two terms we picked to be equal in A are actually equal in A *)
+      rw @similarity_snoc; simpl.
+      exists s1 s2 a a' wa c1; sp.
+      (* easy enough *)
+    }
 
-  assert (lsubstc (subst B x (mk_var z)) wfct1 (snoc s1 (z, a)) pC0
-          = substc a x (lsubstc_vars B wb (csub_filter s1 [x]) [x] c2)) as eq1.
-  rewrite substc_eq_lsubstc; simpl.
-  apply lsubstc_eq_if_csubst.
-  rewrite csubst_app.
-  unfold subst, csubst.
-  try (rw lsubstn_lsubst; try (complete (simpl; rw disjoint_singleton_r; sp))).
-  rewrite simple_lsubst_lsubst;
-    try (complete (sp; allapply @in_csub2sub; sp));
-    try (complete (simpl; sp; cpx; simpl; apply disjoint_singleton_l; auto)).
-  rewrite lsubst_sub_singleton.
-  rewrite fold_csubst.
-  rewrite csubst_snoc_var;
-    try (complete (allapply @similarity_dom; exrepd; allrw; sp)).
-  rewrite <- csub2sub_app; simpl.
-  rewrite <- snoc_as_append.
-  rewrite <- lsubst_swap;
-    try (complete (sp; allapply @in_csub2sub; sp));
-    try (complete (rewrite @dom_csub_eq; rewrite @dom_csub_csub_filter; rw in_remove_nvars; simpl; sp)).
-  repeat (rewrite <- @csub2sub_cons).
-  repeat (rewrite @fold_csubst).
-  destruct (eq_var_dec z x); subst.
-  (* if they're equal it's easy *)
-  rewrite csubst_cons_trim.
-  rewrite csub_filter_snoc1; sp.
-  (* if they're not: *)
-  rewrite <- csubst_csub_filter with (l := [z]);
-    try (rw disjoint_singleton_r; sp).
-  assert (x <> z) as d by auto; simpl.
-  apply memvar_singleton_diff_r in d; rewrite d.
-  rewrite csub_filter_snoc1; sp.
-  rewrite csubst_cons_trim.
-  rewrite <- csub_filter_app_r; simpl.
-  symmetry.
-  rewrite <- csubst_csub_filter with (l := [z]); simpl;
-    try (rw disjoint_singleton_r; sp).
-  rewrite d.
-  rewrite csub_filter_swap.
-  rewrite <- csub_filter_app_r; sp.
+    (* and again, we keep on using our 1st hypothesis *)
+    exrepd. (* we prove that from e *)
+    clear t; clear_irr.
 
-  rewrite eq1 in e; clear eq1.
+    assert (lsubstc (subst B x (mk_var z)) wfct1 (snoc s1 (z, a)) pC0
+            = substc a x (lsubstc_vars B wb (csub_filter s1 [x]) [x] c2)) as eq1.
+    {
+      rewrite substc_eq_lsubstc; simpl.
+      apply lsubstc_eq_if_csubst.
+      rewrite csubst_app.
+      unfold subst, csubst.
+      try (rw lsubstn_lsubst; try (complete (simpl; rw disjoint_singleton_r; sp))).
+      rewrite simple_lsubst_lsubst;
+        try (complete (sp; allapply @in_csub2sub; sp));
+        try (complete (simpl; sp; cpx; simpl; apply disjoint_singleton_l; auto)).
+      rewrite lsubst_sub_singleton.
+      rewrite fold_csubst.
+      rewrite csubst_snoc_var;
+        try (complete (allapply @similarity_dom; exrepd; allrw; sp)).
+      rewrite <- csub2sub_app; simpl.
+      rewrite <- snoc_as_append.
+      rewrite <- lsubst_swap;
+        try (complete (sp; allapply @in_csub2sub; sp));
+        try (complete (rewrite @dom_csub_eq; rewrite @dom_csub_csub_filter; rw in_remove_nvars; simpl; sp)).
+      repeat (rewrite <- @csub2sub_cons).
+      repeat (rewrite @fold_csubst).
+      destruct (eq_var_dec z x); subst.
+      (* if they're equal it's easy *)
+      rewrite csubst_cons_trim.
+      rewrite csub_filter_snoc1; sp.
+      (* if they're not: *)
+      rewrite <- csubst_csub_filter with (l := [z]);
+        try (rw disjoint_singleton_r; sp).
+      assert (x <> z) as d by auto; simpl.
+      apply memvar_singleton_diff_r in d; rewrite d.
+      rewrite csub_filter_snoc1; sp.
+      rewrite csubst_cons_trim.
+      rewrite <- csub_filter_app_r; simpl.
+      symmetry.
+      rewrite <- csubst_csub_filter with (l := [z]); simpl;
+        try (rw disjoint_singleton_r; sp).
+      rewrite d.
+      rewrite csub_filter_swap.
+      rewrite <- csub_filter_app_r; sp.
+    }
 
-  lsubst_tac; sp.
+    rewrite eq1 in e0; clear eq1.
 
-  assert (cequivc lib
-            (lsubstc b wfce1 (snoc s1 (z, a)) pt0)
-            (mkc_apply
-               (mkc_lam z (lsubstc_vars b wfce1 (csub_filter s1 [z]) [z] c0))
-               a)) as ceq1.
-  apply cequivc_sym.
-  revert c0; rw @csub_filter_trivial; introv;
-  try (complete (simpl; sp; subst; allapply @similarity_dom; repnd; allrw sim1; sp)).
-  destruct_cterms; unfold cequivc; simpl; unfold csubst; simpl.
-  allrw @csub2sub_snoc; simpl.
-  generalize (cequiv_beta lib z (lsubst b (csub2sub s1)) x1); introv ceq1.
-  autodimp ceq1 hyp.
-  apply csubst.isprog_vars_lsubst.
-  introv k; allrw @in_range_iff; exrepnd; allapply @in_csub2sub; sp.
-  simpl.
-  rw @isprog_vars_eq; sp.
-  allunfold @covered.
-  rw @dom_csub_eq.
-  allapply @similarity_dom; repnd; allrw.
-  apply subvars_trans with (vs2 := snoc (nh_vars_hyps H) z); sp.
-  rw subvars_prop; introv j; allsimpl; allrw in_snoc; sp.
-  generalize (subset_hs_vars_hyps H); intro k.
-  right; apply k; sp.
-  rw @nt_wf_eq; sp.
-  autodimp ceq1 hyp.
-  allrw @isprogram_eq; sp.
-  rw @simple_lsubst_snoc in ceq1; sp.
-  rw @isprogram_eq; sp.
-  allapply @in_csub2sub; sp.
+    lsubst_tac; sp.
 
-  assert (cequivc lib
-            (lsubstc b wfce1 (snoc s2 (z, a')) pt3)
-            (mkc_apply
-               (mkc_lam z (lsubstc_vars b wfce1 (csub_filter s2 [z]) [z] c3))
-               a'))
-         as ceq2.
-  apply cequivc_sym.
-  revert c3; rw @csub_filter_trivial; introv;
-  try (complete (simpl; sp; subst; allapply @similarity_dom; repnd; allrw sim; sp)).
-  destruct_cterms; unfold cequivc; simpl; unfold csubst; simpl.
-  allrw @csub2sub_snoc; simpl.
-  generalize (cequiv_beta lib z (lsubst b (csub2sub s2)) x0); introv ceq2.
-  autodimp ceq2 hyp.
-  apply csubst.isprog_vars_lsubst.
-  introv k; allrw @in_range_iff; exrepnd; allapply @in_csub2sub; sp.
-  simpl.
-  rw @isprog_vars_eq; sp.
-  allunfold @covered.
-  rw @dom_csub_eq.
-  allapply @similarity_dom; repnd; allrw.
-  apply subvars_trans with (vs2 := snoc (nh_vars_hyps H) z); sp.
-  rw subvars_prop; introv j; allsimpl; allrw in_snoc; sp.
-  generalize (subset_hs_vars_hyps H); intro k.
-  right; apply k; sp.
-  rw @nt_wf_eq; sp.
-  autodimp ceq2 hyp.
-  allrw @isprogram_eq; sp.
-  rw @simple_lsubst_snoc in ceq2; sp.
-  rw @isprogram_eq; sp.
-  allapply @in_csub2sub; sp.
+    assert (cequivc lib
+                    (lsubstc b wfce1 (snoc s1 (z, a)) pt0)
+                    (mkc_apply
+                       (mkc_lam z (lsubstc_vars b wfce1 (csub_filter s1 [z]) [z] c0))
+                       a)) as ceq1.
+    {
+      apply cequivc_sym.
+      revert c0; rw @csub_filter_trivial; introv;
+        try (complete (simpl; sp; subst; allapply @similarity_dom; repnd; allrw sim1; sp)).
+      destruct_cterms; unfold cequivc; simpl; unfold csubst; simpl.
+      allrw @csub2sub_snoc; simpl.
+      generalize (cequiv_beta lib z (lsubst b (csub2sub s1)) x1); introv ceq1.
+      autodimp ceq1 hyp.
+      apply csubst.isprog_vars_lsubst.
+      introv k; allrw @in_range_iff; exrepnd; allapply @in_csub2sub; sp.
+      simpl.
+      rw @isprog_vars_eq; sp.
+      allunfold @covered.
+      rw @dom_csub_eq.
+      allapply @similarity_dom; repnd; allrw.
+      apply subvars_trans with (vs2 := snoc (nh_vars_hyps H) z); sp.
+      rw subvars_prop; introv j; allsimpl; allrw in_snoc; sp.
+      generalize (subset_hs_vars_hyps H); intro k.
+      right; apply k; sp.
+      rw @nt_wf_eq; sp.
+      autodimp ceq1 hyp.
+      allrw @isprogram_eq; sp.
+      rw @simple_lsubst_snoc in ceq1; sp.
+      rw @isprogram_eq; sp.
+      allapply @in_csub2sub; sp.
+    }
 
-  apply @equality_respects_cequivc_left with (t1 := lsubstc b wfce1 (snoc s1 (z, a)) pt0); sp.
-  apply @equality_respects_cequivc_right with (t2 := lsubstc b wfce1 (snoc s2 (z, a')) pt3); sp.
+    assert (cequivc lib
+                    (lsubstc b wfce1 (snoc s2 (z, a')) pt3)
+                    (mkc_apply
+                       (mkc_lam z (lsubstc_vars b wfce1 (csub_filter s2 [z]) [z] c3))
+                       a'))
+      as ceq2.
+    {
+      apply cequivc_sym.
+      revert c3; rw @csub_filter_trivial; introv;
+        try (complete (simpl; sp; subst; allapply @similarity_dom; repnd; allrw sim; sp)).
+      destruct_cterms; unfold cequivc; simpl; unfold csubst; simpl.
+      allrw @csub2sub_snoc; simpl.
+      generalize (cequiv_beta lib z (lsubst b (csub2sub s2)) x0); introv ceq2.
+      autodimp ceq2 hyp.
+      apply csubst.isprog_vars_lsubst.
+      introv k; allrw @in_range_iff; exrepnd; allapply @in_csub2sub; sp.
+      simpl.
+      rw @isprog_vars_eq; sp.
+      allunfold @covered.
+      rw @dom_csub_eq.
+      allapply @similarity_dom; repnd; allrw.
+      apply subvars_trans with (vs2 := snoc (nh_vars_hyps H) z); sp.
+      rw subvars_prop; introv j; allsimpl; allrw in_snoc; sp.
+      generalize (subset_hs_vars_hyps H); intro k.
+      right; apply k; sp.
+      rw @nt_wf_eq; sp.
+      autodimp ceq2 hyp.
+      allrw @isprogram_eq; sp.
+      rw @simple_lsubst_snoc in ceq2; sp.
+      rw @isprogram_eq; sp.
+      allapply @in_csub2sub; sp.
+    }
+
+    apply @equality_respects_cequivc_left with (t1 := lsubstc b wfce1 (snoc s1 (z, a)) pt0); sp.
+    apply @equality_respects_cequivc_right with (t2 := lsubstc b wfce1 (snoc s2 (z, a')) pt3); sp.
+  }
 Qed.
 
 (* begin hide *)
 
 Lemma rule_lambda_formation_true_ex {p} :
-  forall lib i z A B b x H (bc1 : !LIn z (bound_vars B)),
-    @rule_true_if p lib (rule_lambda_formation A B b x z i H).
+  forall lib i z A B b e x H (bc1 : !LIn z (bound_vars B)),
+    @rule_true_if p lib (rule_lambda_formation A B b e x z i H).
 Proof.
   intros.
-  generalize (rule_lambda_formation_true lib A B b x z i H bc1); intro rt.
+  generalize (rule_lambda_formation_true lib A B b e x z i H bc1); intro rt.
   rw <- @rule_true_eq_ex in rt.
   unfold rule_true_ex in rt; sp.
 Qed.
-
-
-
-(* end hide *)
-
 
 (* [24] ============ FUNCTION EQUALITY ============ *)
 
@@ -1228,67 +688,75 @@ Qed.
  *)
 
 Definition rule_function_equality {p}
-           (a1 a2 b1 b2 : NTerm)
+           (a1 a2 b1 b2 e1 e2 : NTerm)
            (x1 x2 y : NVar)
            (i   : nat)
            (H   : @barehypotheses p) :=
   mk_rule
     (mk_baresequent
        H
-       (mk_conclax (mk_equality
-                      (mk_function a1 x1 b1)
-                      (mk_function a2 x2 b2)
-                      (mk_uni i))))
-    [ mk_baresequent
-        H
-        (mk_conclax (mk_equality a1 a2 (mk_uni i))),
+       (mk_concl_eq (mk_function a1 x1 b1)
+                    (mk_function a2 x2 b2)
+                    (mk_uni i)))
+    [ mk_baresequent H (mk_concl_eq_ext a1 a2 (mk_uni i) e1),
       mk_baresequent
         (snoc H (mk_hyp y a1))
-        (mk_conclax (mk_equality
-                       (subst b1 x1 (mk_var y))
-                       (subst b2 x2 (mk_var y))
-                       (mk_uni i)))
+        (mk_concl_eq_ext (subst b1 x1 (mk_var y))
+                         (subst b2 x2 (mk_var y))
+                         (mk_uni i)
+                         e2)
     ]
-    [ sarg_var y ].
+    [ sarg_var y , sarg_term (mk_function a1 x1 b1) ].
 
-Lemma rule_function_equality_true {pp} :
-  forall lib (a1 a2 b1 b2 : NTerm),
-  forall x1 x2 y : NVar,
-  forall i   : nat,
-  forall H   : @barehypotheses pp,
-    rule_true lib (rule_function_equality
-                     a1 a2 b1 b2
+Lemma rule_function_equality_true3 {o} :
+  forall lib (a1 a2 b1 b2 e1 e2 : NTerm)
+         (x1 x2 y : NVar)
+         (i   : nat)
+         (H   : @barehypotheses o),
+    rule_true3 lib (rule_function_equality
+                     a1 a2 b1 b2 e1 e2
                      x1 x2 y
                      i
                      H).
 Proof.
   intros.
-  apply (rule_tyfam_equality_true _ _ mkc_function); auto.
+  apply (rule_tyfam_equality_true3 _ _ mkc_function).
 
   - introv; simpl; allrw remove_nvars_nil_l; allrw app_nil_r; auto.
 
   - introv; apply lsubstc_mk_function_ex.
 
-  - introv; apply equality_function.
+  - apply implies_tequalityi_function; auto.
 Qed.
 
+Lemma rule_function_equality_true {o} :
+  forall lib (a1 a2 b1 b2 e1 e2 : NTerm)
+         (x1 x2 y : NVar)
+         (i   : nat)
+         (H   : @barehypotheses o),
+    rule_true lib (rule_function_equality
+                     a1 a2 b1 b2 e1 e2
+                     x1 x2 y
+                     i
+                     H).
+Proof.
+  introv.
+  apply rule_true3_implies_rule_true.
+  apply rule_function_equality_true3.
+Qed.
 
 (* begin hide *)
 
 
 Lemma rule_function_equality_true_ex {o} :
-  forall lib y i a1 a2 b1 b2 x1 x2 H,
-    @rule_true_if o lib (rule_function_equality a1 a2 b1 b2 x1 x2 y i H).
+  forall lib y i a1 a2 b1 b2 e1 e2 x1 x2 H,
+    @rule_true_if o lib (rule_function_equality a1 a2 b1 b2 e1 e2 x1 x2 y i H).
 Proof.
   intros.
-  generalize (rule_function_equality_true lib a1 a2 b1 b2 x1 x2 y i H); intro rt.
+  generalize (rule_function_equality_true lib a1 a2 b1 b2 e1 e2 x1 x2 y i H); intro rt.
   rw <- @rule_true_eq_ex in rt.
   unfold rule_true_ex in rt; sp.
 Qed.
-
-
-
-(* end hide *)
 
 
 (* [25] ============ LAMBDA EQUALITY ============ *)
@@ -1309,37 +777,36 @@ Qed.
  *)
 
 Definition rule_lambda_equality {o}
-           (A B t1 t2 : NTerm)
+           (A B t1 t2 e1 e2 : NTerm)
            (x1 x2 x z : NVar)
            (i : nat)
            (H : @barehypotheses o) :=
   mk_rule
     (mk_baresequent
        H
-       (mk_conclax (mk_equality
-                      (mk_lam x1 t1)
-                      (mk_lam x2 t2)
-                      (mk_function A x B))))
+       (mk_concl_eq (mk_lam x1 t1)
+                    (mk_lam x2 t2)
+                    (mk_function A x B)))
     [ mk_baresequent
         (snoc H (mk_hyp z A))
-        (mk_conclax (mk_equality
-                       (subst t1 x1 (mk_var z))
-                       (subst t2 x2 (mk_var z))
-                       (subst B x (mk_var z)))),
+        (mk_concl_eq_ext (subst t1 x1 (mk_var z))
+                         (subst t2 x2 (mk_var z))
+                         (subst B x (mk_var z))
+                         e1),
       mk_baresequent
         H
-        (mk_conclax (mk_equality A A (mk_uni i))) ]
+        (mk_concl_eq_ext A A (mk_uni i) e2) ]
     [sarg_var z].
 
 Lemma rule_lambda_equality_true {o} :
-  forall lib (A B t1 t2 : NTerm)
+  forall lib (A B t1 t2 e1 e2 : NTerm)
          (x1 x2 x z : NVar)
          (i   : nat)
          (H   : @barehypotheses o)
          (bc1 : !LIn z (bound_vars B))
          (bc2 : !LIn z (bound_vars t1))
          (bc3 : !LIn z (bound_vars t2)),
-    rule_true lib (rule_lambda_equality A B t1 t2 x1 x2 x z i H).
+    rule_true lib (rule_lambda_equality A B t1 t2 e1 e2 x1 x2 x z i H).
 Proof.
   intros.
   unfold rule_lambda_equality, rule_true, closed_type_baresequent, closed_extract_baresequent; simpl.
@@ -1361,7 +828,12 @@ Proof.
   duplicate ce0 as ce.
   allrw @nh_vars_hyps_snoc; allsimpl.
 
-  exists (@covered_axiom o (nh_vars_hyps H)); GC.
+  match goal with
+  | [ |- context[covered ?a ?b] ] => assert (covered a b) as covc
+  end.
+  {
+    clear hyp1 hyp2.
+  }
 
   (* We prove some simple facts on our sequents *)
   assert ((z <> x -> !LIn z (free_vars B))
@@ -1592,12 +1064,6 @@ Proof.
   rewrite eq in hyp0; clear eq.
   auto.
 Qed.
-
-(* begin hide *)
-
-
-
-(* end hide *)
 
 (* [26] ============ APPLY @EQUALITY ============ *)
 
@@ -2366,5 +1832,642 @@ Proof.
   introv e.
   generalize (eqlam a a' s1 s1 eqh sim1); intro k; exrepnd; clear_irr; sp.
 Qed.
+
+
+
+(* end hide *)
+
+(**
+
+  The Nuprl manual%~\cite{Kreitz:02}% presents various useful rules to
+  reason about function types.  This section prove the truth of
+  several of these rules.
+
+*)
+
+(* [17] ============ FUNCTION ELIMINATION ============ *)
+
+(**
+
+ The following rule is called the function elimination rules.  It says
+ that if we can prove that [a] is in the domain [A] then we can assume
+ that [f a] is in [B[x\a]].  As for the other rules, first we show an
+ informal statement of this rule, then we show its formal statement (a
+ [Definition]), and finally we show the statement that the rule is
+ true (a [Lemma]).  In such informal statements, we write ``C ext e''
+ to indicate that e is the extract of the sequent, i.e., the evidence
+ that C is true.  We omit the ``ext e'' part when e is [mk_axiom].
+
+<<
+   H, f : x:A->B[x], J |- C ext e[z\(f a)]
+
+     By functionElimination s z
+
+     H, f : x:A->B[x], J |- a in A
+     H, f : x:A->B[x], J, z : (f a) in B[a] |- C ext e
+>>
+
+ *)
+
+Definition rule_function_elimination_concl {o}
+           (A : @NTerm o) B C a e f x z H J :=
+  mk_baresequent
+    (snoc H (mk_hyp f (mk_function A x B)) ++ J)
+    (mk_concl C (subst e z (mk_apply (mk_var f) a))).
+
+Definition rule_function_elimination_hyp1 {o}
+           (A : @NTerm o) B a ea f x H J :=
+  mk_baresequent
+    (snoc H (mk_hyp f (mk_function A x B)) ++ J)
+    (mk_concl (mk_member a A) ea).
+
+Definition rule_function_elimination_hyp2 {o}
+           (A : @NTerm o) B C a e f x z H J :=
+  mk_baresequent
+    (snoc (snoc H (mk_hyp f (mk_function A x B)) ++ J)
+          (mk_hyp z (mk_member (mk_apply (mk_var f) a)
+                               (subst B x a))))
+    (mk_concl C e).
+
+Definition rule_function_elimination {p}
+           (A B C a e : NTerm) ea
+           (f x z : NVar)
+           (H J : @barehypotheses p) :=
+  mk_rule
+    (rule_function_elimination_concl A B C a e f x z H J)
+    [
+      rule_function_elimination_hyp1 A B a ea f x H J,
+      rule_function_elimination_hyp2 A B C a e f x z H J
+    ]
+    [ sarg_term a (*, sarg_var z*)].
+
+Lemma rule_function_elimination_true3 {p} :
+  forall lib (A B C a e : NTerm) ea
+         (f x z : NVar)
+         (H J : @barehypotheses p),
+    rule_true3 lib (rule_function_elimination
+                      A B C a e
+                      ea
+                      f x z
+                      H J).
+Proof.
+  unfold rule_function_elimination, rule_true3, wf_bseq, closed_type_baresequent, closed_extract_baresequent; simpl.
+  intros; repnd.
+
+  pose proof (cargs (sarg_term a)) as ca.
+  simpl in ca; autodimp ca hyp.
+  rw @nh_vars_hyps_app in ca; simpl in ca.
+  rw @nh_vars_hyps_snoc in ca; simpl in ca.
+
+  (* We prove the well-formedness of things *)
+  destseq; allsimpl.
+  dLin_hyp; exrepnd.
+  rename Hyp into hyp1.
+  rename Hyp0 into hyp2.
+  destruct hyp1 as [ ws1 hyp1 ].
+  destruct hyp2 as [ ws2 hyp2 ].
+  destseq; allsimpl; proof_irr; GC.
+
+  assert (wf_csequent (rule_function_elimination_concl A B C a e f x z H J)) as wfc.
+  {
+    clear hyp1 hyp2.
+    unfold wf_csequent, closed_type, closed_extract, wf_sequent, wf_concl; simpl.
+    prove_seq; eauto 3 with slow.
+    { apply wf_term_subst; eauto 3 with slow.
+      apply wf_apply; eauto 2 with slow. }
+    apply covered_subst; eauto 2 with slow.
+    { eapply covered_subvars;[|eauto].
+      autorewrite with slow; simpl.
+      rw subvars_eq; introv i; simpl.
+      repeat (allrw @in_snoc; allrw @in_app_iff).
+      repndors; tcsp. }
+    { apply covered_apply; dands; eauto 3 with slow.
+      apply covered_var; rw in_app_iff; rw in_snoc; tcsp. }
+  }
+  exists wfc.
+  unfold wf_csequent, wf_sequent, wf_concl in wfc; allsimpl; repnd; proof_irr; GC.
+
+  (* We prove some simple facts on our sequents *)
+  assert (disjoint (free_vars A) (vars_hyps J)
+          # disjoint (remove_nvars [x] (free_vars B)) (vars_hyps J)
+          # subvars (free_vars a) (snoc (vars_hyps H) f ++ vars_hyps J)
+          # wf_term a
+          # !LIn z (free_vars C)
+          # !LIn z (vars_hyps H)
+          # !LIn z (vars_hyps J)
+          # (z <> f)
+          # !LIn f (vars_hyps H)
+          # !LIn f (vars_hyps J)
+          # !LIn f (free_vars A)
+          # (x <> f -> !LIn f (free_vars B))) as vhyps.
+  {
+    clear hyp1 hyp2.
+    dwfseq.
+    sp;
+      try (complete (introv i; discover; allunfold @disjoint; discover; auto));
+      try (complete (assert (LIn f (remove_nvars [x] (free_vars B)))
+                      by (rw in_remove_nvars; rw in_single_iff; sp);
+                     discover; auto));
+      try (complete (apply wf_member_iff in wfct0; sp));
+      try (complete (generalize (wfh10 z); rw in_app_iff; rw in_snoc; sp));
+      try (complete (generalize (wfh10 f); rw in_remove_nvars; simpl; intro i;
+                     dest_imp i hyp));
+      try complete (pose proof (wfc1 z) as xx; autodimp xx hyp;
+                    rw in_app_iff in xx; rw in_snoc in xx; repndors; tcsp).
+  }
+
+  destruct vhyps as [ daj vhyps ].
+  destruct vhyps as [ dbj vhyps ].
+  destruct vhyps as [ sva vhyps ].
+  destruct vhyps as [ wa vhyps ].
+  destruct vhyps as [ nizc vhyps ].
+  destruct vhyps as [ nizh vhyps ].
+  destruct vhyps as [ nizj vhyps ].
+  destruct vhyps as [ nzf vhyps ].
+  destruct vhyps as [ nifh vhyps ].
+  destruct vhyps as [ nifj vhyps ].
+  destruct vhyps as [ nifa nifb ].
+  (* done with proving these simple facts *)
+
+  vr_seq_true.
+
+  duplicate sim as simapp.
+
+  rw @similarity_app in sim; simpl in sim; exrepnd; subst; cpx.
+  rw @similarity_snoc in sim5; simpl in sim5; exrepnd; subst; cpx.
+  lsubst_tac.
+  rw @equality_in_function in sim2; repnd.
+
+  vr_seq_true in hyp2.
+
+  assert (cover_vars a (snoc s1a0 (f, t1) ++ s1b)) as cova1.
+  {
+    apply cover_vars_eq.
+    rw @dom_csub_app; rw @dom_csub_snoc; simpl.
+    clear hyp1; revert ct0.
+    unfold covered; simpl; autorewrite with slow.
+    repeat (rw @subvars_app_l).
+    introv h; repnd; clear h; GC.
+    rw @vars_hyps_app in h0; rw @vars_hyps_snoc in h0; simpl in h0.
+    apply similarity_dom in sim6; repnd; allrw.
+    apply similarity_dom in sim1; repnd; allrw.
+    autorewrite with slow; auto.
+  }
+
+  assert (cover_vars a (snoc s2a0 (f, t2) ++ s2b)) as cova2.
+  {
+    apply cover_vars_eq.
+    rw @dom_csub_app; rw @dom_csub_snoc; simpl.
+    clear hyp1; revert ct0.
+    unfold covered; simpl; autorewrite with slow.
+    repeat (rw @subvars_app_l).
+    introv h; repnd; clear h; GC.
+    rw @vars_hyps_app in h0; rw @vars_hyps_snoc in h0; simpl in h0.
+    apply similarity_dom in sim6; repnd; allrw.
+    apply similarity_dom in sim1; repnd; allrw.
+    autorewrite with slow; auto.
+  }
+
+  generalize (hyp2 (snoc (snoc s1a0 (f, t1) ++ s1b)
+                         (z, mkc_prefl (mkc_apply t1 (lsubstc a wa (snoc s1a0 (f, t1) ++ s1b) cova1))
+                                       (mkc_apply t1 (lsubstc a wa (snoc s1a0 (f, t1) ++ s1b) cova1))))
+                   (snoc (snoc s2a0 (f, t2) ++ s2b)
+                         (z, mkc_prefl (mkc_apply t2 (lsubstc a wa (snoc s2a0 (f, t2) ++ s2b) cova2))
+                                       (mkc_apply t2 (lsubstc a wa (snoc s2a0 (f, t2) ++ s2b) cova2)))));
+    clear hyp2; intros hyp2.
+  repeat (autodimp hyp2 h); exrepnd.
+
+  {
+    (* hyps_functionality *)
+
+    apply hyps_functionality_snoc2; simpl; auto;[].
+    introv equ sim; GC; lsubst_tac.
+
+    apply equality_in_member in equ.
+    exrepnd; computes_to_value_isvalue.
+
+    assert (equality lib (lsubstc a wa (snoc s1a0 (f, t1) ++ s1b) cova1)
+                     (lsubstc a wa s' c4)
+                     (lsubstc A w1 s1a0 c1)) as eqa.
+    {
+      vr_seq_true in hyp1.
+      generalize (hyp1 (snoc s1a0 (f, t1) ++ s1b) s'); clear hyp1; intros hyp1.
+      repeat (autodimp hyp1 h); exrepnd.
+      lsubst_tac.
+      allapply @member_if_inhabited.
+      apply tequality_mkc_member_implies_equality in hyp0; auto.
+    }
+
+    apply implies_tequality_mkc_member_if_member.
+
+    {
+      duplicate sim as sim'.
+      apply eqh in sim'.
+      rw @eq_hyps_app in sim'; simpl in sim'; exrepnd; subst; cpx.
+      apply app_split in sim'0; repnd; allrw length_snoc;
+        try (complete (allrw; sp)); subst; cpx.
+
+      rw @eq_hyps_snoc in sim'5; simpl in sim'5; exrepnd; subst; cpx.
+      lsubst_tac.
+      rw @tequality_function in sim'0; repnd.
+
+    }
+
+    vr_seq_true in hyp1.
+    generalize (hyp1 (snoc s1a0 (f, t1) ++ s1b) s'); clear hyp1; intros hyp1.
+    repeat (autodimp hyp1 h); exrepnd.
+    lsubst_tac.
+    allapply @member_if_inhabited.
+    rw @tequality_mkc_member_sp in hyp0; repnd.
+
+    assert (equality lib (lsubstc a wa (snoc s1a0 (f, t1) ++ s1b) c3)
+                     (lsubstc a wa s' c5)
+                     (lsubstc A w1 s1a0 c1)) as eqa.
+    {
+      sp.
+      unfold member in hyp1.
+      spcast; apply @equality_respects_cequivc_right with (t2 := lsubstc a wa (snoc s1a0 (f, t1) ++ s1b) c3); sp.
+    }
+
+    applydup sim5 in eqa.
+
+    duplicate sim as sim'.
+    apply eqh in sim'.
+
+    rw @eq_hyps_app in sim'; simpl in sim'; exrepnd; subst; cpx.
+    apply app_split in sim'0; repnd; allrw length_snoc;
+    try (complete (allrw; sp)); subst; cpx.
+
+    rw @eq_hyps_snoc in sim'5; simpl in sim'5; exrepnd; subst; cpx.
+    lsubst_tac.
+    rw @tequality_function in sim'0; repnd.
+
+    applydup sim'0 in eqa as teq.
+
+    assert (disjoint (remove_nvars [x] (free_vars B)) (dom_csub s1b0)) as disj1.
+    {
+      apply similarity_dom in sim1; repnd.
+      rw sim7.
+      rewrite vars_hyps_substitute_hyps; auto.
+    }
+
+    assert (disjoint (remove_nvars [x] (free_vars B)) (dom_csub s2b0)) as disj2.
+    {
+      apply sub_eq_hyps_dom in sim'1; repnd.
+      rw sim'1; auto.
+    }
+
+    repeat (substc_lsubstc_vars3;[]).
+
+    dands.
+
+    {
+      repeat (lsubstc_subst_aeq2;[]).
+      repeat (substc_lsubstc_vars3;[]).
+      repeat (lsubstc_weak;[]).
+      proof_irr.
+      auto.
+    }
+
+    rw @similarity_app in sim; simpl in sim; exrepnd; subst; cpx.
+    apply app_split in sim7; repnd; allrw length_snoc;
+    try (complete (allrw; sp)); subst; cpx.
+    apply app_split in sim9; repnd; allrw length_snoc;
+    try (complete (allrw; sp)); subst; cpx.
+    rw @similarity_snoc in sim12; simpl in sim12; exrepnd; subst; cpx.
+    lsubst_tac.
+    rw @equality_in_function in sim9; repnd.
+    applydup sim9 in eqa as eqf.
+
+    left.
+    repeat (lsubstc_subst_aeq2;[]).
+    repeat (substc_lsubstc_vars3;[]).
+    repeat (lsubstc_weak;[]).
+    proof_irr.
+    auto.
+  }
+
+
+  {
+    (* similarity *)
+
+    assert (wf_term (mk_member (mk_apply (mk_var f) a) (subst B x a))) as wm.
+    {
+      apply wf_member; sp; try (apply wf_apply; sp).
+      apply subst_preserves_wf_term; sp.
+    }
+
+    assert (cover_vars (mk_member (mk_apply (mk_var f) a) (subst B x a))
+                       (snoc s1a0 (f, t1) ++ s1b)) as cm.
+    {
+      apply cover_vars_member; sp.
+      apply cover_vars_apply; sp.
+      apply cover_vars_var.
+      rw @dom_csub_app; rw @dom_csub_snoc; rw in_app_iff; rw in_snoc; simpl; sp.
+      rw @cover_vars_eq; rw @dom_csub_app; rw @dom_csub_snoc; insub.
+      (* begin proof of last cover_vars *)
+      rw @cover_vars_eq; rw @cover_vars_covered; apply covered_subst; sp.
+      rw @dom_csub_app; rw @dom_csub_snoc; simpl.
+      rw cons_app; apply covered_app_weak_l.
+      clear sim2 sim5; unfold cover_vars_upto in c2; unfold covered.
+      prove_subvars c2; allsimpl; sp.
+      rw @dom_csub_csub_filter in l; rw in_remove_nvars in l; rw in_single_iff in l.
+      rw in_snoc; sp.
+      clear hyp1; rw @covered_equality in ct0; repnd.
+      unfold covered; unfold covered in ct1.
+      rw @vars_hyps_app in ct1; rw @vars_hyps_snoc in ct1; simpl in ct1.
+      rw @dom_csub_app; rw @dom_csub_snoc; simpl.
+      allapply @similarity_dom; repnd; allrw; rw @vars_hyps_substitute_hyps; sp.
+      (* end proof of last cover_vars *)
+    }
+
+    sim_snoc.
+    dands; auto.
+    lsubst_tac.
+    rw @member_eq.
+    rw <- @member_member_iff.
+
+    vr_seq_true in hyp1.
+    generalize (hyp1 (snoc s1a0 (f, t1) ++ s1b)
+                     (snoc s2a0 (f, t2) ++ s2b));
+      clear hyp1; intros hyp1.
+    repeat (autodimp hyp1 h); exrepnd.
+    lsubst_tac.
+    allapply @member_if_inhabited.
+    rw @tequality_mkc_member_sp in hyp0; repnd.
+    unfold member in hyp1.
+    apply sim2 in hyp1.
+
+    assert (disjoint (remove_nvars [x] (free_vars B)) (dom_csub s1b)) as disj1.
+    {
+      apply similarity_dom in sim1; repnd.
+      rw sim7.
+      rewrite vars_hyps_substitute_hyps; auto.
+    }
+
+    apply equality_refl in hyp1.
+    unfold member in *.
+    repeat (lsubstc_subst_aeq2;[]).
+    repeat (substc_lsubstc_vars3;[]).
+    repeat (lsubstc_weak;[]).
+    proof_irr.
+    auto.
+  }
+
+  (* conclusion *)
+
+  lsubst_tac; sp.
+
+  assert (wf_term (@mk_axiom p)) as wfax by eauto 2 with slow.
+
+  repeat (lsubstc_subst_aeq2;[]).
+  allrw @lsubstc_mk_axiom.
+  repeat (substc_lsubstc_vars3;[]).
+  proof_irr.
+
+  pose proof (lsubstc_snoc_move
+                e
+                (snoc s1a0 (f, t1) ++ s1b)
+                []
+                z
+                mkc_axiom
+                wfce) as xx1.
+  allrw app_nil_r.
+  allrw @dom_csub_app.
+  allrw @dom_csub_snoc.
+  allsimpl.
+  pose proof (xx1 pt0) as xx2; clear xx1.
+  autodimp xx2 hyp.
+  { apply similarity_dom in sim6; repnd.
+    rewrite sim7.
+    apply similarity_dom in sim1; repnd.
+    rewrite sim8.
+    rewrite vars_hyps_substitute_hyps; auto.
+    rw in_app_iff; rw in_snoc; intro i; repndors; tcsp.
+  }
+  exrepnd.
+  proof_irr.
+  rewrite <- xx0; clear xx0.
+
+  pose proof (lsubstc_snoc_move
+                e
+                (snoc s2a0 (f, t2) ++ s2b)
+                []
+                z
+                mkc_axiom
+                wfce) as xx1.
+  allrw app_nil_r.
+  allrw @dom_csub_app.
+  allrw @dom_csub_snoc.
+  allsimpl.
+  pose proof (xx1 pt3) as xx2; clear xx1.
+  autodimp xx2 hyp.
+  { apply similarity_dom in sim6; repnd.
+    rewrite sim6.
+    apply similarity_dom in sim1; repnd.
+    rewrite sim1.
+    rewrite vars_hyps_substitute_hyps; auto.
+    rw in_app_iff; rw in_snoc; intro i; repndors; tcsp.
+  }
+  exrepnd.
+  proof_irr.
+  rewrite <- xx0; clear xx0.
+
+  auto.
+Qed.
+
+(* begin hide *)
+
+Lemma rule_function_elimination_true {p} :
+  forall lib (A B C a e : NTerm) ea,
+  forall f x z : NVar,
+  forall H J : @barehypotheses p,
+    rule_true lib (rule_function_elimination
+                     A B C a e
+                     ea
+                     f x z
+                     H J).
+Proof.
+  introv.
+  apply rule_true3_implies_rule_true.
+  apply rule_function_elimination_true3.
+Qed.
+
+Lemma rule_function_elimination_true2 {o} :
+  forall lib A B C a e ea f x z H J,
+    @rule_true2 o lib (rule_function_elimination A B C a e ea f x z H J).
+Proof.
+  intros.
+  apply rule_true_iff_rule_true2.
+  apply rule_function_elimination_true.
+Qed.
+
+Lemma rule_function_elimination_true_ex {p} :
+  forall lib (A B C a e : NTerm) ea,
+  forall f x z : NVar,
+  forall H J : @barehypotheses p,
+    rule_true_if lib (rule_function_elimination
+                        A B C a e
+                        ea
+                        f x z
+                        H J).
+Proof.
+  intros.
+  generalize (rule_function_elimination_true lib A B C a e ea f x z H J); intro rt.
+  rw <- @rule_true_eq_ex in rt.
+  unfold rule_true_ex in rt; sp.
+Qed.
+
+Lemma rule_function_elimination_wf {o} :
+  forall (A B C a e : @NTerm o) ea f x z H J,
+    wf_term a
+    -> covered a (snoc (vars_hyps H) f ++ vars_hyps J)
+    -> !LIn z (vars_hyps H)
+    -> !LIn z (vars_hyps J)
+    -> z <> f
+    -> wf_term ea
+    -> wf_rule (rule_function_elimination A B C a e ea f x z H J).
+Proof.
+  introv wa cov nizH nizJ dzf wea.
+
+  introv pwf m; allsimpl; repdors; subst; sp;
+  allunfold @pwf_sequent; wfseq; sp.
+
+  {
+    allrw @vswf_hypotheses_nil_eq.
+    allrw @wf_hypotheses_app; repnd.
+    allrw @wf_hypotheses_snoc; repnd.
+    allsimpl.
+    allapply @isprog_vars_implies_wf.
+    allrw <- @wf_function_iff; tcsp.
+  }
+
+  {
+    allrw @vswf_hypotheses_nil_eq.
+    allrw @wf_hypotheses_app; repnd.
+    allrw @wf_hypotheses_snoc; repnd.
+    allsimpl.
+    allapply @isprog_vars_implies_covered.
+    allrw @covered_function; repnd.
+    apply covered_snoc_app_weak.
+    apply covered_app_weak_l; auto.
+  }
+
+  {
+    allrw @vswf_hypotheses_nil_eq.
+    rw @wf_hypotheses_snoc; simpl; dands; tcsp.
+    - apply isprog_vars_member; dands.
+      + apply isprog_vars_apply; dands.
+        * apply isprog_vars_var_iff.
+          rw @vars_hyps_app.
+          rw @vars_hyps_snoc; simpl.
+          rw in_app_iff.
+          rw in_snoc; tcsp.
+        * rw @isprog_vars_iff_covered; dands; auto.
+          rw @vars_hyps_app.
+          rw @vars_hyps_snoc; simpl; auto.
+      + apply isprog_vars_subst2; auto.
+        * allrw @wf_hypotheses_app; repnd.
+          allrw @wf_hypotheses_snoc; repnd.
+          allsimpl.
+          allapply @isprog_vars_implies_wf.
+          allrw <- @wf_function_iff; tcsp.
+        * rw @isprog_vars_iff_covered; dands; auto.
+          rw @vars_hyps_app.
+          rw @vars_hyps_snoc; simpl; auto.
+        * allrw @wf_hypotheses_app; repnd.
+          allrw @wf_hypotheses_snoc; repnd.
+          allsimpl.
+          allrw <- @isprog_vars_function_iff; repnd.
+          allrw @vars_hyps_app.
+          allrw @vars_hyps_snoc; simpl.
+          eapply isprog_vars_subvars;[|eauto].
+          rw subvars_eq; introv i; allsimpl.
+          allrw in_app_iff; allrw in_snoc; tcsp.
+    - intro i.
+      allrw @vars_hyps_app.
+      allrw @vars_hyps_snoc; allsimpl.
+      allrw in_app_iff; allrw in_snoc.
+      repndors; tcsp.
+  }
+
+  {
+    allrw @wf_term_eq.
+    allrw @nt_wf_lsubst_iff; tcsp.
+  }
+
+  {
+    apply covered_snoc_weak; auto.
+  }
+Qed.
+
+Lemma rule_function_elimination_wf2 {o} :
+  forall (A B C a e : @NTerm o) ea f x z H J,
+    wf_term a
+    -> covered a (snoc (vars_hyps H) f ++ vars_hyps J)
+    -> !LIn z (vars_hyps H)
+    -> !LIn z (vars_hyps J)
+    -> z <> f
+    -> wf_rule2 (rule_function_elimination A B C a e ea f x z H J).
+Proof.
+  introv wa cova nizH nizJ dzf wf j.
+  allsimpl; repndors; subst; tcsp;
+  allunfold @wf_bseq; repnd; allsimpl; wfseq.
+
+  - allrw @vswf_hypotheses_nil_eq.
+    allrw @wf_hypotheses_app; repnd.
+    allrw @wf_hypotheses_snoc; repnd.
+    allapply @isprog_vars_implies_wf.
+    allrw <- @wf_function_iff; tcsp.
+
+  - allrw @vswf_hypotheses_nil_eq.
+    allrw @wf_hypotheses_app; repnd.
+    allrw @wf_hypotheses_snoc; repnd.
+    allapply @isprog_vars_implies_covered.
+    allrw @covered_function; repnd.
+    apply covered_snoc_app_weak.
+    apply covered_app_weak_l; auto.
+
+  - allrw @vswf_hypotheses_nil_eq.
+    rw @wf_hypotheses_snoc; simpl; dands; tcsp.
+    { apply isprog_vars_member; dands.
+      + apply isprog_vars_apply; dands.
+        * apply isprog_vars_var_iff.
+          rw @vars_hyps_app.
+          rw @vars_hyps_snoc; simpl.
+          rw in_app_iff.
+          rw in_snoc; tcsp.
+        * rw @isprog_vars_iff_covered; dands; auto.
+          rw @vars_hyps_app.
+          rw @vars_hyps_snoc; simpl; auto.
+      + apply isprog_vars_subst2; auto.
+        * allrw @wf_hypotheses_app; repnd.
+          allrw @wf_hypotheses_snoc; repnd.
+          allsimpl.
+          allapply @isprog_vars_implies_wf.
+          allrw <- @wf_function_iff; tcsp.
+        * rw @isprog_vars_iff_covered; dands; auto.
+          rw @vars_hyps_app.
+          rw @vars_hyps_snoc; simpl; auto.
+        * allrw @wf_hypotheses_app; repnd.
+          allrw @wf_hypotheses_snoc; repnd.
+          allsimpl.
+          allrw <- @isprog_vars_function_iff; repnd.
+          allrw @vars_hyps_app.
+          allrw @vars_hyps_snoc; simpl.
+          eapply isprog_vars_subvars;[|eauto].
+          rw subvars_eq; introv i; allsimpl.
+          allrw in_app_iff; allrw in_snoc; tcsp.
+    }
+    { intro i.
+      allrw @vars_hyps_app.
+      allrw @vars_hyps_snoc; allsimpl.
+      allrw in_app_iff; allrw in_snoc.
+      repndors; tcsp.
+    }
+
+  - apply covered_snoc_weak; auto.
+Qed.
+
 
 (* end hide *)
